a bunch of hashconsing tricks on IPOptionsSmall, and an extra spec benchmark

deps/poulet4/lib/P4automata/Benchmarks/IPOptionsProofSmall.v
@@ -24,17 +24,18 @@ Module SelfComparison.
   Notation A := (Sum.sum IPOptions32.aut IPOptions32.aut).
   Notation conf := (P4automaton.configuration (P4A.interp A)).
 
-
   Definition r_states :=
     Eval vm_compute in (Reachability.reachable_states
                           A
-                          10
+                          5
                           IPOptions32.Parse0
                           IPOptions32.Parse0).
 
-  (* Definition r_with_len := Eval vm_compute in (length r_states, r_states).
+  
 
-  Print r_with_len. *)
+  (* Definition r_len := Eval vm_compute in (length r_states). *)
+
+  (* Print r_len. *)
 
   Definition top : Relations.rel conf := fun _ _ => True.
   Definition top' : Relations.rel (state_template A) := fun _ _ => True.
@@ -51,20 +52,8 @@ Module SelfComparison.
     (  IPOptions32.L1, FirstOrderConfRelSimplified.Bits 8)
     (  IPOptions32.V1, FirstOrderConfRelSimplified.Bits 24).
 
-  Inductive mark : nat -> Type := M : forall (n: nat), mark n.
+  
     
-  Ltac measure_goals := match goal with 
-    | |- pre_bisimulation _ _ _ _ ?R _ _ => 
-      let x := fresh "rem_goals" in
-      pose proof (x := M (length R));
-      vm_compute in x;
-      match goal with 
-      | H : mark ?n |- _ => 
-        idtac "remaining goals: " n;
-        clear H
-      end
-    end.
-
   Lemma prebisim_babyip:
     forall q1 q2,
       interp_conf_rel' {| cr_st := {|
@@ -84,81 +73,192 @@ Module SelfComparison.
                     (wp r_states)
                     top
                     []
-                    (mk_init _ _ _ A 10 IPOptions32.Parse0 IPOptions32.Parse0)
+                    (mk_init _ _ _ A 5 IPOptions32.Parse0 IPOptions32.Parse0)
                     q1 q2.
   Proof.
     idtac "running ipoptions ref self-comparison bisimulation".
 
     intros.
-    set (rel0 := (mk_init _ _ _ A 10 IPOptions32.Parse0 IPOptions32.Parse0)).
+    set (rel0 := (mk_init _ _ _ _ _ _ _)).
     vm_compute in rel0.
     subst rel0.
-    clear H.
+    
+    (* set (seven := 7).
+    assert (H7 : 7 = seven); [subst seven; reflexivity|]. *)
+    set (eight := 8).
+    assert (H8 : 8 = eight); [subst eight; reflexivity|].
+    (* assert (H8' : Datatypes.S seven = eight); [subst; reflexivity|]. *)
+    (* set (fifteen := (Datatypes.S( Datatypes.S( Datatypes.S( Datatypes.S( Datatypes.S( Datatypes.S( Datatypes.S eight)))))))).
+    assert (H15 : ( Datatypes.S( Datatypes.S( Datatypes.S( Datatypes.S( Datatypes.S( Datatypes.S( Datatypes.S eight))))))) = fifteen); [subst fifteen; reflexivity|]. *)
+    set (sixteen := (Datatypes.S( Datatypes.S( Datatypes.S( Datatypes.S( Datatypes.S( Datatypes.S( Datatypes.S( Datatypes.S eight))))))))).
+    assert (H16 : (Datatypes.S( Datatypes.S( Datatypes.S( Datatypes.S( Datatypes.S( Datatypes.S( Datatypes.S( Datatypes.S eight)))))))) = sixteen); [subst sixteen; reflexivity|].
+    (* assert (H16' : (Datatypes.S fifteen = sixteen)); [subst; reflexivity|]. *)
+
+    (* try rewrite H7; *)
+    try rewrite H8;
+    (* try rewrite H15; *)
+    try rewrite H16.
+    (* try rewrite H16'. *)
+
+    match goal with 
+    | |- pre_bisimulation _ _ _ _ ?R _ _ => 
+      hashcons_list R
+    end.
 
     Set Ltac Profiling.
 
-    (* match goal with 
-    | |- pre_bisimulation _ _ _ _ ?G _ _ =>
-      hashcons_list G
-    end. *)
+    time "build phase" repeat (run_bisim top top' r_states;
 
-    (* Set Ltac Profiling. *)
-
-
-
-    do 25 ((time "single step" run_bisim top top' r_states);
-    match goal with 
-    | |- pre_bisimulation _ _ _ (?N :: _) _ _ _  => 
+    try rewrite H8;
+    try rewrite H16;
+    
+    try match goal with 
+    | |- pre_bisimulation _ _ _ (?N :: ?N' :: ?T) _ _ _  => 
+      let rs := fresh "rs" in 
+      set (rs := N' :: T);
       let r := fresh "r" in 
       set (r := N)
-    | _ => idtac
-    end).
-
-    do 25 ((time "single step" run_bisim top top' r_states);
-    match goal with 
-    | |- pre_bisimulation _ _ _ (?N :: _) _ _ _  => 
+      
+    | |- pre_bisimulation _ _ _ (?N :: nil) _ _ _  => 
       let r := fresh "r" in 
       set (r := N)
-    | _ => idtac
     end).
 
-    do 25 ((time "single step" run_bisim top top' r_states);
-    match goal with 
-    | |- pre_bisimulation _ _ _ (?N :: _) _ _ _  => 
-      let r := fresh "r" in 
-      set (r := N)
-    | _ => idtac
-    end).
-
-    do 25 ((time "single step" run_bisim top top' r_states);
-    match goal with 
-    | |- pre_bisimulation _ _ _ (?N :: _) _ _ _  => 
-      let r := fresh "r" in 
-      set (r := N)
-    | _ => idtac
-    end).
-
-    do 25 ((time "single step" run_bisim top top' r_states);
-    match goal with 
-    | |- pre_bisimulation _ _ _ (?N :: _) _ _ _  => 
-      let r := fresh "r" in 
-      set (r := N)
-    | _ => idtac
-    end).
-
-    do 25 ((time "single step" run_bisim top top' r_states);
-    match goal with 
-    | |- pre_bisimulation _ _ _ (?N :: _) _ _ _  => 
-      let r := fresh "r" in 
-      set (r := N)
-    | _ => idtac
-    end).
-
-    idtac "150 steps..., quitting...".
 
     Show Ltac Profile.
+    Reset Ltac Profile.
+
+    time "close phase" close_bisim top'.
+
+    Show Ltac Profile.
+    Reset Ltac Profile.
 
  Time Admitted.
 
 End SelfComparison.
 
+Module SpecCompare.
+    
+  Notation H := (IPOptions32.header + IPOptionsSpec32.header).
+  Notation A := (Sum.sum IPOptions32.aut IPOptionsSpec32.aut).
+  Notation conf := (P4automaton.configuration (P4A.interp A)).
+
+
+  Definition r_states :=
+    Eval vm_compute in (Reachability.reachable_states
+                          A
+                          5
+                          IPOptions32.Parse0
+                          IPOptionsSpec32.Parse0).
+
+  
+
+  (* Definition r_len := Eval vm_compute in (length r_states).
+
+  Print r_len. *)
+
+  Definition top : Relations.rel conf := fun _ _ => True.
+  Definition top' : Relations.rel (state_template A) := fun _ _ => True.
+
+  ClearEnvCtors.
+
+  RegisterEnvCtors
+    (IPOptions32.Scratch8, FirstOrderConfRelSimplified.Bits 8)
+    (  IPOptions32.Scratch16, FirstOrderConfRelSimplified.Bits 16)
+    (  IPOptions32.T0, FirstOrderConfRelSimplified.Bits 8)
+    (  IPOptions32.L0, FirstOrderConfRelSimplified.Bits 8)
+    (  IPOptions32.V0, FirstOrderConfRelSimplified.Bits 24)
+    (  IPOptions32.T1, FirstOrderConfRelSimplified.Bits 8)
+    (  IPOptions32.L1, FirstOrderConfRelSimplified.Bits 8)
+    (  IPOptions32.V1, FirstOrderConfRelSimplified.Bits 24)
+    (IPOptionsSpec32.Scratch8, FirstOrderConfRelSimplified.Bits 8)
+    (  IPOptionsSpec32.Scratch16, FirstOrderConfRelSimplified.Bits 16)
+    (  IPOptionsSpec32.Scratch24, FirstOrderConfRelSimplified.Bits 24)
+    (  IPOptionsSpec32.T0, FirstOrderConfRelSimplified.Bits 8)
+    (  IPOptionsSpec32.L0, FirstOrderConfRelSimplified.Bits 8)
+    (  IPOptionsSpec32.V, FirstOrderConfRelSimplified.Bits 16).
+
+  
+
+  Lemma prebisim_babyip:
+    forall q1 q2,
+      interp_conf_rel' {| cr_st := {|
+                          cs_st1 := {|
+                            st_state := inl (inl (IPOptions32.Parse0));
+                            st_buf_len := 0;
+                          |};
+                          cs_st2 := {|
+                            st_state := inl (inr (IPOptionsSpec32.Parse0));
+                            st_buf_len := 0;
+                          |};
+                        |};
+                        cr_ctx := BCEmp;
+                        cr_rel := btrue;
+                    |} q1 q2 ->
+    pre_bisimulation A
+                    (wp r_states)
+                    top
+                    []
+                    (mk_init _ _ _ A 5 IPOptions32.Parse0 IPOptionsSpec32.Parse0)
+                    q1 q2.
+  Proof.
+    idtac "running ipoptions small specialized bisimulation".
+
+    intros.
+    set (rel0 := (mk_init _ _ _ _ _ _ _)).
+    vm_compute in rel0.
+    subst rel0.
+    
+    (* set (seven := 7).
+    assert (H7 : 7 = seven); [subst seven; reflexivity|]. *)
+    set (eight := 8).
+    assert (H8 : 8 = eight); [subst eight; reflexivity|].
+    (* assert (H8' : Datatypes.S seven = eight); [subst; reflexivity|]. *)
+    (* set (fifteen := (Datatypes.S( Datatypes.S( Datatypes.S( Datatypes.S( Datatypes.S( Datatypes.S( Datatypes.S eight)))))))).
+    assert (H15 : ( Datatypes.S( Datatypes.S( Datatypes.S( Datatypes.S( Datatypes.S( Datatypes.S( Datatypes.S eight))))))) = fifteen); [subst fifteen; reflexivity|]. *)
+    set (sixteen := (Datatypes.S( Datatypes.S( Datatypes.S( Datatypes.S( Datatypes.S( Datatypes.S( Datatypes.S( Datatypes.S eight))))))))).
+    assert (H16 : (Datatypes.S( Datatypes.S( Datatypes.S( Datatypes.S( Datatypes.S( Datatypes.S( Datatypes.S( Datatypes.S eight)))))))) = sixteen); [subst sixteen; reflexivity|].
+    (* assert (H16' : (Datatypes.S fifteen = sixteen)); [subst; reflexivity|]. *)
+
+    (* try rewrite H7; *)
+    try rewrite H8;
+    (* try rewrite H15; *)
+    try rewrite H16.
+    (* try rewrite H16'. *)
+
+    match goal with 
+    | |- pre_bisimulation _ _ _ _ ?R _ _ => 
+      hashcons_list R
+    end.
+
+    Set Ltac Profiling.
+
+    time "build phase" repeat (run_bisim top top' r_states;
+
+    try rewrite H8;
+    try rewrite H16;
+    
+    try match goal with 
+    | |- pre_bisimulation _ _ _ (?N :: ?N' :: ?T) _ _ _  => 
+      let rs := fresh "rs" in 
+      set (rs := N' :: T);
+      let r := fresh "r" in 
+      set (r := N)
+      
+    | |- pre_bisimulation _ _ _ (?N :: nil) _ _ _  => 
+      let r := fresh "r" in 
+      set (r := N)
+    end).
+
+
+    Show Ltac Profile.
+    Reset Ltac Profile.
+
+    time "close phase" close_bisim top'.
+
+    Show Ltac Profile.
+    Reset Ltac Profile.
+
+ Time Admitted.
+
+End SpecCompare.
